@prefix : <http://data.cimple.eu/ontology#> .
@prefix cimple: <http://data.cimple.eu/ontology/> .
@prefix owl: <http://www.w3.org/2002/07/owl#> .
@prefix rdf: <http://www.w3.org/1999/02/22-rdf-syntax-ns#> .
@prefix schema: <http://schema.org/> .
@prefix rdfs: <http://www.w3.org/2000/01/rdf-schema#> .
@prefix vann: <http://purl.org/vocab/vann/> .
@prefix skos: <http://www.w3.org/2004/02/skos/core#> .

<http://data.cimple.eu/ontology#> rdf:type owl:Ontology ;
                                  vann:preferredNamespaceUri "http://data.cimple.eu/ontology/" ;
                                  dc:creator <http://data.cimple.eu>;

#################################################################
#    Object Properties
#################################################################

###  http://data.cimple.eu/ontology#credibility_score
cimple:credibility_score rdf:type owl:ObjectProperty ;
                         rdfs:domain schema:CreativeWork ;
                         rdfs:comment """This property indicates the credibility score of an instance of CreativeWork

Examples:
* TODO"""@en .

###  http://data.cimple.eu/ontology#hasEmotion
cimple:hasEmotion rdf:type owl:ObjectProperty ;
                  rdfs:domain schema:CreativeWork ;
                  rdfs:range skos:Concept ;
                  rdfs:comment """This property indicates that an instance of CreativeWork has the spcified emotion

Examples:
* TODO"""@en .

###  http://data.cimple.eu/ontology#hasPoliticalLeaning
cimple:hasPoliticalLeaning rdf:type owl:ObjectProperty ;
                           rdfs:domain schema:CreativeWork ;
                           rdfs:range skos:Concept ;
                           rdfs:comment """This property indicates that an instance of CreativeWork has the spcified political leaning

Examples:
* TODO"""@en .

###  http://data.cimple.eu/ontology#hasSentiment
cimple:hasSentiment rdf:type owl:ObjectProperty ;
                    rdfs:domain schema:CreativeWork ;
                    rdfs:comment """This property indicates that an instance of CreativeWork has the spcified sentiment

Examples:
* TODO"""@en .

###  http://data.cimple.eu/ontology#mentionsConspiracy
cimple:mentionsConspiracy rdf:type owl:ObjectProperty ;
                          rdfs:domain schema:CreativeWork ;
                          rdfs:range skos:Concept ;
                          rdfs:comment """This property indicates that an instance of CreativeWork mentions the spcified conspiracy theory

Examples:
* TODO"""@en .

###  http://data.cimple.eu/ontology#promotesConspiracy
cimple:promotesConspiracy rdf:type owl:ObjectProperty ;
                          rdfs:domain schema:CreativeWork ;
                          rdfs:range skos:Concept ;
                          rdfs:comment """This property indicates that an instance of CreativeWork promotes the spcified conspiracy theory

Examples:
* TODO"""@en .

###  http://data.cimple.eu/ontology#normalizedReviewRating
cimple:normalizedReviewRating rdf:type owl:ObjectProperty ;
                              rdfs:domain schema:ClaimReview ;
                              rdfs:range schema:Rating ;
                              rdfs:comment """This property indicates that an instance of ClaimReview has the specified normalized review rating

Examples:
* TODO"""@en .

###  http://data.cimple.eu/ontology#related
cimple:related rdf:type owl:ObjectProperty ;
               rdfs:domain schema:CreativeWork ;
               rdfs:range schema:CreativeWork ;
               rdfs:comment """This property indicates that two instance of ClaimReviews are related

Examples:
* TODO"""@en .

